Simple_Firewall/SimpleFw_Compliance.thy
@@ -1,5 +1,5 @@
 theory SimpleFw_Compliance
-imports SimpleFw_Semantics "../Primitive_Matchers/IPPortIfaceSpace_Matcher" "../Semantics_Ternary" "../Output_Format/Negation_Type_Matching"
+imports SimpleFw_Semantics "../Primitive_Matchers/IPPortIfaceSpace_Matcher" "../Semantics_Ternary" "../Output_Format/Negation_Type_Matching" "../Bitmagic/Numberwang_Ln"
 begin
 
 fun ipv4_word_netmask_to_nattuple :: "(ipv4addr \<times> nat)  \<Rightarrow> ipt_ipv4range" where
@@ -22,7 +22,7 @@ fun simple_match_to_ipportiface_match :: "simple_match \<Rightarrow> ipportiface
 
 
 (*is this usefull?*)
-lemma "matches \<gamma> (simple_match_to_ipportiface_match \<lparr>iiface=iif, oiface=oif, src=sip, dst=dip, proto=p, sports=sps, dports=dps \<rparr>) a p \<longleftrightarrow> 
+lemma xxx: "matches \<gamma> (simple_match_to_ipportiface_match \<lparr>iiface=iif, oiface=oif, src=sip, dst=dip, proto=p, sports=sps, dports=dps \<rparr>) a p \<longleftrightarrow> 
       matches \<gamma> (alist_and ([Pos (IIface iif), Pos (OIface oif)] @ (NegPos_map (Src \<circ> ipv4_word_netmask_to_nattuple) [sip])
         @ (NegPos_map (Dst \<circ> ipv4_word_netmask_to_nattuple) [dip]) @ [Pos (Prot p)]
         @ (NegPos_map (\<lambda>x. Src_Ports [x]) [sps]) @ (NegPos_map (\<lambda>x. Dst_Ports [x]) [dps]))) a p"
@@ -37,11 +37,56 @@ apply(case_tac [!] dps)
 apply(simp_all add: bunch_of_lemmata_about_matches)
 done
 
+(*TODO: smelly duplication*)
+lemma matches_Src_simple_match: "matches (ipportiface_matcher, \<alpha>) (negation_type_to_match_expr (\<lambda>x. ipportiface_rule_match.Src (ipv4_word_netmask_to_nattuple x)) ip) a p \<longleftrightarrow>
+  simple_match_ip ip (p_src p)"
+apply(cases ip)
+ apply(rename_tac i_ip)
+ apply(case_tac i_ip)
+ apply(rename_tac iip n)
+ apply(simp add: bunch_of_lemmata_about_matches ternary_to_bool_bool_to_ternary ipv4addr_of_dotteddecimal_dotteddecimal_of_ipv4addr)
+apply(simp)
+apply(rename_tac i_ip)
+apply(case_tac i_ip)
+apply(rename_tac iip n)
+apply(simp add: matches_case_ternaryvalue_tuple split: ternaryvalue.split)
+apply(simp add: bunch_of_lemmata_about_matches bool_to_ternary_simps ipv4addr_of_dotteddecimal_dotteddecimal_of_ipv4addr)
+done
+lemma matches_Dst_simple_match: "matches (ipportiface_matcher, \<alpha>) (negation_type_to_match_expr (\<lambda>x. ipportiface_rule_match.Dst (ipv4_word_netmask_to_nattuple x)) ip) a p \<longleftrightarrow>
+  simple_match_ip ip (p_dst p)"
+apply(cases ip)
+ apply(rename_tac i_ip)
+ apply(case_tac i_ip)
+ apply(rename_tac iip n)
+ apply(simp add: bunch_of_lemmata_about_matches ternary_to_bool_bool_to_ternary ipv4addr_of_dotteddecimal_dotteddecimal_of_ipv4addr)
+apply(simp)
+apply(rename_tac i_ip)
+apply(case_tac i_ip)
+apply(rename_tac iip n)
+apply(simp add: matches_case_ternaryvalue_tuple split: ternaryvalue.split)
+apply(simp add: bunch_of_lemmata_about_matches bool_to_ternary_simps ipv4addr_of_dotteddecimal_dotteddecimal_of_ipv4addr)
+done
+
+
+lemma ports_to_set_singleton_simple_match_port: "p \<in> ports_to_set [a] \<longleftrightarrow> simple_match_port (Pos a) p"
+  by(cases a, simp)
+
+
 lemma "matches (ipportiface_matcher, \<alpha>) (simple_match_to_ipportiface_match sm) a p \<longleftrightarrow> simple_matches sm p"
-  apply(simp add: matches_case_ternaryvalue_tuple bool_to_ternary_Unknown bool_to_ternary_simps split: ternaryvalue.split)
   apply(cases sm)
-  thm eval_ternary_simps bool_to_ternary_simps
-  (*TODO*: ternary_ternary_eval_simps*)
-  apply(safe)
+  apply(rename_tac iif oif sip dip pro sps dps)
+  apply(simp add: bunch_of_lemmata_about_matches ternary_to_bool_bool_to_ternary)
+  apply(rule refl_conj_eq)+
+  apply(simp add: matches_Src_simple_match matches_Dst_simple_match)
+  apply(rule refl_conj_eq)+
+(*brute force proof from here*)
+apply(case_tac [!] sps)
+apply(simp_all)
+apply(case_tac [!] dps)
+apply(simp_all)
+apply(simp_all add: bunch_of_lemmata_about_matches eval_ternary_simps ternary_to_bool_bool_to_ternary)
+apply(simp_all add: ports_to_set_singleton_simple_match_port)
+apply(auto simp add: matches_case_ternaryvalue_tuple bunch_of_lemmata_about_matches bool_to_ternary_simps split: ternaryvalue.split) (\<otimes>h dear, sorry for that*)
+done
 
 end
