Ternary.thy
@@ -112,7 +112,7 @@ by (simp add: eval_ternary_And_comm)
 
 lemma "eval_ternary_Not (ternary_ternary_eval t) = (ternary_ternary_eval (TernaryNot t))" by simp
 
-lemma eval_ternary_simps: 
+lemma eval_ternary_simps_simple: 
   "eval_ternary_And TernaryTrue x = x"
   "eval_ternary_And x TernaryTrue = x"
   "eval_ternary_And TernaryFalse x = TernaryFalse"
@@ -120,6 +120,21 @@ lemma eval_ternary_simps:
 by(case_tac [!] x)(simp_all)
 
 
+lemma eval_ternary_simps_2: "eval_ternary_And (bool_to_ternary P) T = TernaryTrue \<longleftrightarrow> P \<and> T = TernaryTrue"
+      "eval_ternary_And T (bool_to_ternary P) = TernaryTrue \<longleftrightarrow> P \<and> T = TernaryTrue"
+  apply(case_tac [!] P)
+  apply(simp_all add: eval_ternary_simps_simple)
+  done
+
+lemma eval_ternary_simps_3: "eval_ternary_And (ternary_ternary_eval x) T = TernaryTrue \<longleftrightarrow> (ternary_ternary_eval x = TernaryTrue) \<and> (T = TernaryTrue)"
+      "eval_ternary_And T (ternary_ternary_eval x) = TernaryTrue \<longleftrightarrow> (ternary_ternary_eval x = TernaryTrue) \<and> (T = TernaryTrue)"
+  apply(case_tac [!] T)
+  apply(simp_all add: eval_ternary_simps_simple)
+  apply(case_tac [!] "(ternary_ternary_eval x)")
+  apply(simp_all)
+  done
+
+lemmas eval_ternary_simps = eval_ternary_simps_simple eval_ternary_simps_2 eval_ternary_simps_3
 
 definition ternary_eval :: "ternaryformula \<Rightarrow> bool option" where
   "ternary_eval t = ternary_to_bool (ternary_ternary_eval t)"
